\documentclass[a4j,10pt]{jarticle}
\setlength{\hoffset}{-1.4in}
\setlength{\voffset}{-0.9in}
\renewcommand{\arraystretch}{2}
\renewcommand{\tabcolsep}{-5.0mm}
\usepackage{prelude}
\usepackage{booktabs}
\pagestyle{empty}
\def\FTransform#1{\simbol\left[#1\right]}
\def\Fourier{\def\simbol{\mathcal F}
  \def\t{t} \def\f{f} \def\ft{\f(\t)}
            \def\g{g} \def\gt{\g(\t)}
  \def\w{\omega} \def\F{F} \def\Fw{\F(\w)}
                 \def\G{G} \def\Gw{\G(\w)}
  \def\Transform{\FTransform}
}
\def\LTransform#1{\simbol\left[#1\right]}
\def\Laplace{\def\simbol{\mathcal L}
  \def\t{t} \def\f{f} \def\ft{\f(\t)}
            \def\g{g} \def\gt{\g(\t)}
  \def\w{s} \def\F{F} \def\Fw{\F(\w)}
            \def\G{G} \def\Gw{\G(\w)}
  \def\Transform{\LTransform}
}
\def\ZTransform#1{\simbol\left[#1\right]}
\def\Ztrans{\def\simbol{\mathcal Z}
  \def\t{n} \def\f{x} \def\ft{\f[\t]}
            \def\g{y} \def\gt{\g[\t]}
  \def\w{z} \def\F{X} \def\Fw{\F(\w)}
            \def\G{Y} \def\Gw{\G(\w)}
  \def\Transform{\ZTransform}
}
\def\Br{\mathrm{Br}}
\def\jj{i}
\def\ii{i}
\def\iii#1#2{\int_{-\infty}^\infty#2\dd#1}
\def\sii#1#2{\sum_{#1=-\infty}^\infty#2}
\def\izi#1#2{\int_0^\infty#2\dd#1}
\def\szi#1#2{\sum_{#1=0}^\infty#2}
\def\ds{\displaystyle}
\def\convolution#1#2{#1*#2}
\def\kakeru#1#2{#1#2}
\def\linearsum#1#2{a#1+b#2}
\def\sgn{\mathrm{sgn}}
\def\entry#1#2#3{\Fourier#1&\Laplace#2&\Ztrans#3\\}

\begin{document}
\begin{table}[htbp]
\begin{tabular}{ccc}
\toprule
\entry
{\LARGE$\simbol$}
{\LARGE$\simbol$}
{\LARGE$\simbol$}
\hline\hline
\entry
{$\ds \Fw = \iii\t{\ft\ee^{-\jj\w\t}}$}
{$\ds \Fw = \izi\t{\ft\ee^{-   \w\t}}$}
{$\ds \Fw = \szi\t{\ft\w^{-\t}}$}
\entry
{$\ds \ft = \frac 1 {2\pi   } \iii\w{\Fw\ee^{\jj\w\t}}$}
{$\ds \ft = \frac 1 {2\pi\ii} \int_\Br\Fw\ee^{\w\t}\dd\w$}
{$\ds \ft = \frac 1 {2\pi\ii} \oint_C\Fw\w^{\t-1}\dd\w$}
\hline
\entry
{$\ds $}
{$\ds \ft = 0 \;(\t < 0)$}
{$\ds \ft = 0 \;(\t < 0)$}
\entry
{$\ds \Transform{\ft} = \Fw$}
{$\ds \Transform{\ft} = \Fw$}
{$\ds \Transform{\ft} = \Fw$}
\entry
{$\ds \Transform{\linearsum\ft\gt} = \linearsum\Fw\Gw$}
{$\ds \Transform{\linearsum\ft\gt} = \linearsum\Fw\Gw$}
{$\ds \Transform{\linearsum\ft\gt} = \linearsum\Fw\Gw$}
\entry
{$\ds \Transform{\f(\t-\t_0)} = \Fw\ee^{-\jj\w\t_0}$}
{$\ds \Transform{\f(\t-\t_0)} = \Fw\ee^{-   \t_0\w}$}
{$\ds \Transform{\f[\t-\t_0]} = \Fw\w^{-\t_0}$}
\entry
{$\ds \Transform{\ft\ee^{\jj\w_0\t}} = \F\paren{\w-\w_0}$}
{$\ds \Transform{\ft\ee^{   \w_0\t}} = \F\paren{\w-\w_0}$}
{$\ds \Transform{\ft{\w_0}^\t} = \F\paren{\w/\w_0}$}
\entry
{$\ds \Transform{\f(a\t)} = \frac 1 {\abs a}\F\paren{\frac\w a}$}
{$\ds \Transform{\f(a\t)} = \frac 1 {\abs a}\F\paren{\frac\w a}$}
{}
\entry
{$\ds \Transform{\F(\t)} = 2\pi\f(-\w)$}
{}
{}
\entry
{$\ds \Transform{\diffn[n]\ft\t} = \paren{\jj\w}^n\Fw$}
{$\ds \Transform{\diffn[n]\ft\t} = \w^n\Fw-\sum_{k=0}^{n-1}s^{n-k-1}\f^{(k)}(+0)$}
{$\ds \Transform{\f[\t]-\f[\t-1]} = \frac\Fw{1-\w^{-1}}$}
\entry
{$\ds \Transform{\t^n\ft} = \jj^n\diffn[n]\Fw\w$}
{$\ds \Transform{\t^n\ft} = (-1)^n\diffn[n]\Fw\w$}
{$\ds \Transform{\t\ft} = -\w\diff\Fw\w$ }
\entry
{$\ds \Transform{\convolution\ft\gt} = \kakeru\Fw\Gw$}
{$\ds \Transform{\convolution\ft\gt} = \kakeru\Fw\Gw$}
{$\ds \Transform{\convolution\ft\gt} = \kakeru\Fw\Gw$}
\entry
{$\ds \Transform{\kakeru\ft\gt} = \frac 1 {2\pi} \convolution\Fw\Gw$}
{$\ds \Transform{\kakeru\ft\gt} = \frac 1 {2\pi\jj} \lim_{T\to\infty}{\int_{c-iT}^{c+iT}\F(\sigma)\G(\w-\sigma)\dd\sigma}$}
{$\ds \Transform{\kakeru\ft\gt} = \frac 1 {2\pi\jj} {\oint_C\F(\sigma)\G(\w/\sigma)\sigma^{-1}\dd\sigma}$}
\entry
{$\ds \convolution\ft\gt = \iii\tau{\f(\tau)\g(\t-\tau)}$}
{$\ds \convolution\ft\gt = \int_0^t{\f(\tau)\g(\t-\tau)}\dd\tau$}
{$\ds \convolution\ft\gt = \sii m {\f[m]\g[\t-m]}$}
\hline
\entry
{$\ds \Transform{\delta(\t)} = 1$}
{$\ds \Transform{\delta(\t)} = 1$}
{$\ds \Transform{\delta[\t]} = 1$}
\entry
{$\ds \Transform{1} = 2\pi\delta(\w)$}
{$\ds \Transform{1} = \frac 1 \w$}
{$\ds \Transform{1} = \frac 1 {1-\w^{-1}}$}
\entry
{$\ds \Transform{\t} = -2\pi\jj\frac{\delta(\w)}{\w}$}
{$\ds \Transform{\t} = \frac{1}{\w^2}$}
{$\ds \Transform{\t T} = \frac{T\w^{-1}}{\paren{1-\w^{-1}}^2}$}
\entry
{$\ds \Transform{\t^k} = 2\pi\jj^k\delta^{(k)}(\w)$}
{$\ds \Transform{\t^k} = \frac{k!}{\w^{k+1}}$}
{$\ds \Transform{\paren{\t T}^k} = \left[ \diffn[k]{}{s}\frac 1 {\paren{1-\w^{-1}\ee^{sT}}}\right]\Bigg|_{s=0}$}
\entry
{$\ds \Transform{\ee^{\jj\w_0\t}} = 2\pi\delta(\w-\w_0)$}
{$\ds \Transform{\ee^{   \w_0\t}} = \frac 1 {\w-\w_0}$}
{$\ds \Transform{\ee^{\alpha\t T}} = \frac 1 {1 - z^{-1}\ee^{\alpha T}}$}
\entry
{$\ds \Transform{\sin{\beta\t}} = -\jj\pi\paren{\delta\paren{\w-\beta}-\delta\paren{\w+\beta}}$}
{$\ds \Transform{\sin{\beta\t}} = \frac{\beta}{\w^2+\beta^2}$}
{$\ds \Transform{\sin{\beta\t T}} = \frac{\w^{-1}\sin{\beta T}}{1-2\w^{-1}\cos{\beta T}+\w^{-2}}$}
\entry
{$\ds \Transform{\cos{\beta\t}} = \pi\paren{\delta\paren{\w-\beta}+\delta\paren{\w+\beta}}$}
{$\ds \Transform{\cos{\beta\t}} = \frac{\w}{\w^2+\beta^2}$}
{$\ds \Transform{\cos{\beta\t T}} = \frac{1-\w^{-1}\cos{\beta T}}{1-2\w^{-1}\cos{\beta T}+\w^{-2}}$}
\entry
{$\ds \Transform{\Pi{\paren{\t/T}}} = T{\sin\frac{\w T}{2}}\Big/{\frac{\w T}{2}}$}
{$\ds \Transform{\Pi_{T_1}^{T_2}{\paren{\t}}} = \frac 1 \w \paren{\ee^{-\w T_1}-\ee^{-\w T_2}}$}
{}
\bottomrule
\end{tabular}
\end{table}

\end{document}

